(Single-instance) FORS-TW specification.

FORS_TW.ec
@@ -1,7 +1,7 @@
 (* - Require/Import - *)
 (* -- Built-In (Standard Library) -- *)
-require import AllCore List Distr FinType BitEncoding.
-(*---*) import BS2Int.
+require import AllCore List Distr FinType IntDiv BitEncoding.
+(*---*) import BS2Int BitChunking.
 
 
 (* -- Local -- *)
@@ -13,18 +13,18 @@ require (*--*) KeyedHashFunctions TweakableHashFunctions HashAddresses.
 (* - Parameters - *)
 (* -- General -- *)
 (* Length of addresses used in tweakable hash functions (including unspecified global/context part) *)
-const adrs_len : { int | 4 <= adrs_len} as ge4_adrslen.
+const adrs_len : { int | 5 <= adrs_len} as ge4_adrslen.
 
 (* Byte-length of each private key element, public key element, and signature element *)
 const n : { int | 1 <= n } as ge1_n.
 
-(* Number of private key sets and merkle trees *)
+(* Number of private key sets and Merkle trees *)
 const k : { int | 1 <= k } as ge1_k.
 
-(* Height of each merkle tree *)
+(* Height of each Merkle tree *)
 const a : { int | 1 <= a } as ge1_a.
 
-(* Number of elements in each private key set and leaves in each merkle tree *)
+(* Number of elements in each private key set and leaves in each Merkle tree *)
 const t : int = 2 ^ a.
 
 (* Address type constant for tree hashing *)
@@ -34,36 +34,66 @@ const trhtype : int.
 const trcotype : int.
 
 
-(* -- Notions -- *)
-(*  Number of FORS-TW instances to consider in security notion *)
-const d : { int | 1 <= d } as ge1_d.
+(* -- Instances -- *)
+(* 
+  Number of FORS-TW instances in a keypair set 
+  (SPHINCS+: Number of leaves of single XMSS instance on bottom layer)  
+*)
+const l : { int | 1 <= l } as ge1_l.
+
+(* 
+  Number of keypair sets 
+  (SPHINCS+: Number of XMSS instance on bottom layer)  
+*)
+const s : { int | 1 <= s } as ge1_s. 
+
+(* Number of FORS-TW instances to consider *)
+const d : int = s * l.
 
 
 (* -- Properties of parameters -- *)
 (* The different address types are distinct *)
 axiom dist_adrstypes : trhtype <> trcotype. 
 
-(* t is greater than or equal to 2 *)
+(* 
+  Number of leaves of a Merkle tree in a FORS-TW instance is 
+  greater than or equal to 2 
+*)
 lemma ge2_t : 2 <= t.
 proof. by rewrite /t -{1}expr1 StdOrder.IntOrder.ler_weexpn2l 2:ge1_a. qed. 
+
+(* 
+  Number of FORS-TW instances is greater than or equal to 1
+*)
+lemma ge1_d : 1 <= d.
+proof. by rewrite /d StdOrder.IntOrder.mulr_ege1 1:ge1_s ge1_l. qed.
 
 
 
 (* - Types (1/2) - *)
 (* -- General -- *)
-(*
+(* Instance index *)
+clone import Subtype as InstanceIndex with
+  type T <- int,
+    op P i <- 0 <= i < d
+    
+  proof *.
+  realize inhabited by exists 0; smt(ge1_d).
+
+type iid = InstanceIndex.sT.
+  
 (* Randomness for message compression *)
 type mkey.
-*)
+
 (* Secret seeds *)
 type sseed.
 
 (* Public seeds *)
 type pseed.
-(*
+
 (* Messages *)
 type msg = bool list.
-*)
+
 (* 
   Digests, i.e., outputs of (tweakable) hash functions. 
   In fact, also input of (tweakable) hash functions in this case.
@@ -112,8 +142,8 @@ type pkFORS = dgstblock.
 
 (* Secret keys *)
 clone import Subtype as SkFORS with
-  type T   <- dgstblock list,
-    op P l <- size l = k * t
+  type T <- dgstblock list,
+    op P ls <- size ls = k * t
     
   proof *.
   realize inhabited by exists (nseq (k * t) witness); smt(size_nseq ge1_k ge2_t).
@@ -121,8 +151,8 @@ clone import Subtype as SkFORS with
 type skFORS = SkFORS.sT.
 
 clone import Subtype as MsgFORSTW with
-  type T   <- bool list,
-    op P l <- size l = k * a
+  type T <- bool list,
+    op P ls <- size ls = k * a
     
   proof *.
   realize inhabited by exists (nseq (k * a) witness); smt(size_nseq ge1_k ge1_a).
@@ -132,18 +162,18 @@ type msgFORSTW = MsgFORSTW.sT.
 (* Lists of length a containing digests with length 1 (block of 8 * n bits) *)
 clone import Subtype as DBAL with
   type T   <- dgstblock list,
-    op P l <- size l = a
+    op P ls <- size ls = a
     
   proof *.
   realize inhabited by exists (nseq a witness); smt(size_nseq ge1_a).
    
-(* Authentication paths in merkle trees *)
+(* Authentication paths in Merkle trees *)
 type apFORSTW = DBAL.sT.
 
 (* Lists of length k containing skFORSTW (single element)/apFORSTW pairs *)
 clone import Subtype as DBAPKL with
   type T   <- (dgstblock * apFORSTW) list,
-    op P l <- size l = k
+    op P ls <- size ls = k
     
   proof *.
   realize inhabited by exists (nseq k witness); smt(size_nseq ge1_k).
@@ -155,26 +185,42 @@ type sigFORSTW = DBAPKL.sT.
 
 (* - Operators (1/2) - *)
 (* -- Auxiliary -- *)
-(* Number of nodes in a merkle tree (of total height a) at a particular height a' *)
+(* Number of nodes in a Merkle tree (of total height a) at a particular height a' *)
 op nr_nodes (a' : int) = 2 ^ (a - a').
 
 
 (* -- Validity checks -- *)
+(* Tree (keypair set) index validity check *)
+op valid_tidx (tidx : int) : bool =
+  0 <= tidx < s.
+
 (* Type index validity check *)
 op valid_typeidx (typeidx : int) : bool =
   typeidx = trhtype \/ typeidx = trcotype.
 
 (* Keypair index validity check *)
 op valid_kpidx (kpidx : int) : bool = 
-  0 <= kpidx < k.
+  0 <= kpidx < l.
 
 (* Tree height index validity check *)
 op valid_thidx (thidx : int) : bool = 
   0 <= thidx <= a.
 
-(* Tree breadth index validity check *)
-op valid_tbidx (thidx tbidx : int) : bool = 
-  0 <= tbidx < nr_nodes thidx.
+(* 
+  Tree breadth index validity check.
+  Note that, according to the specs, this index is not reset
+  across Merkle trees in a FORS-TW instance. E.g.,
+  the breadth index of the left-most leaf of the i-th tree (out of k)
+  has breadth index i * t; the left-most node of the i-th tree at
+  height 1 has breadth index i * (t // 2); and the root node of the
+  i-th tree has breadth index i. In other words, the left-most node of 
+  a certain layer in the i-th tree is given the incremented breadth index
+  from the right-most node at the same layer of the (i - 1)-th tree.
+  The generic formula for the breadth index of a node at height j in the
+  i-th tree should thus be i * (t // 2 ^ j).
+*)
+op valid_tbidx (thidx tbidx : int) : bool =
+  0 <= tbidx < k * nr_nodes thidx.
 
 (* Overall (generic) validity check for indices of addresses *)
 op valid_idxvals : int list -> bool.
@@ -194,14 +240,16 @@ op valid_fidxvalslptrh (adidxs : int list) : bool =
      valid_tbidx (nth witness adidxs 1) (nth witness adidxs 0)
   /\ valid_thidx (nth witness adidxs 1)
   /\ valid_kpidx (nth witness adidxs 2)
-  /\ nth witness adidxs 3 = trhtype.
-
+  /\ nth witness adidxs 3 = trhtype
+  /\ valid_tidx (nth witness adidxs 4).
+  
 (* Tree root compression address indices validity check (local part) *)
 op valid_fidxvalslptrco (adidxs : int list) : bool = 
      nth witness adidxs 0 = 0
   /\ nth witness adidxs 1 = 0
   /\ valid_kpidx (nth witness adidxs 2)
-  /\ nth witness adidxs 3 = trcotype.
+  /\ nth witness adidxs 3 = trcotype
+  /\ valid_tidx (nth witness adidxs 4).
    
 (* 
   Validity check for the local part of the indices corresponding to a FORS-TW address
@@ -246,6 +294,9 @@ qed.
 
 
 (* - Distributions - *)  
+(* Proper distribution over randomness for message compression *)
+op [lossless] dmkey : mkey distr.
+
 (* Proper distribution over public seeds *)
 op [lossless] dpseed : pseed distr.
 
@@ -299,6 +350,9 @@ proof. smt(valid_fadrsidxs_adrsidxs). qed.
 
 
 (* -- Setters -- *)
+op set_tidx (ad : adrs) (i : int) : adrs =
+  set_idx ad 4 i.
+  
 op set_typeidx (ad : adrs) (i : int) : adrs =
   insubd (put (put (put (put (val ad) 0 0) 1 0) 2 0) 3 i).
 
@@ -308,16 +362,136 @@ op set_kpidx (ad : adrs) (i : int) : adrs =
 op set_thtbidx (ad : adrs) (i j : int) : adrs =
   insubd (put (put (val ad) 0 j) 1 i).
 
+
+(* -- Getters -- *)
+op get_kpidx (ad : adrs) : int =
+  get_idx ad 2.
   
+
+(* -- Keyed Hash Functions -- *)
+(* Secret key element generation function *)
+op skg : sseed -> (pseed * adrs) -> dgstblock.
+
+clone KeyedHashFunctions as SKG with
+  type key_t <- sseed,
+  type in_t <- pseed * adrs,
+  type out_t <- dgstblock,
+  
+    op f <- skg
+    
+  proof *.
+
+clone import SKG.PRF as SKG_PRF with
+  op dkey <- dsseed,
+  op doutm d <- ddgstblock
+  
+  proof *.
+  realize dkey_ll by exact: dsseed_ll.
+  realize doutm_ll by move => d; apply ddgstblock_ll. 
+  
+
+(* --- Message compression --- *)
+(* Message compression function *)
+op mco : mkey -> msg -> msgFORSTW * iid.
+
+(* 
+  Function mapping output of message compression function to a list
+  containing three-tuples of which the entries respectively signify the following.
+  - The index of a key set (i.e., pointer to a specific FORS-TW instance).
+  - The index of a secret value set (i.e., pointer to Merkle tree in FORS-TW instance indicated by first value of tuple). 
+  - The index of a secret value (i.e., pointer to a leaf of the Merkle tree indicated by second value of tuple). 
+*)
+op g (mi : msgFORSTW * iid) : (int * int * int) list =
+  let cmsg = chunk a (val mi.`1) in
+  let iidx = val mi.`2 in
+    mkseq (fun (i : int) => (iidx, i, bs2int (rev (nth witness cmsg i)))) k.
+
+clone KeyedHashFunctions as MCO with
+  type key_t <- mkey,
+  type in_t <- msg,
+  type out_t <- msgFORSTW * iid,
+  
+    op f <- mco
+    
+  proof *.
+  
+clone import MCO.ITSR as MCO_ITSR with  
+  op ks <- d,
+  op svsks <- k,
+  op svsvs <- t,
+  
+  op g <- g,
+  
+  op dkey <- dmkey
+  
+  proof *.
+  realize ge1_ks by exact: ge1_d.
+  realize ge1_svsks by exact: ge1_k.
+  realize ge1_svsvs by smt(ge2_t).
+  realize size_g by move=> mi @/g /=; rewrite size_mkseq; smt(ge1_k).
+  realize rng_iks. by move => x mi @/g /= /mkseqP [i] [_ ->] /=; rewrite valP. qed.
+  realize rng_sv.
+    move=> x mi @/g /= /mkseqP [i] [rng_i -> /=].
+    rewrite bs2int_ge0 /= /t; pose r := rev _.
+    suff ->: a = size r; 1: by rewrite bs2int_le2Xs.
+    rewrite /r size_rev. search size nth.
+    have: all (((=) a) \o size) (chunk a (val mi.`1)).
+    + rewrite allP => bs bsin.
+      by rewrite /(\o) eq_sym (in_chunk_size a (val mi.`1)) //; smt(ge1_a).
+    move/all_nthP => /= /(_ witness i _) //.
+    by rewrite size_chunk 2:valP 2:mulzK; smt(ge1_a).
+  qed.
+  realize eqiks_g. by move=> x x' mi @/g /= /mkseqP [?] [? ->] /mkseqP [?] [? ->]. qed.
+  realize neqisvs_g. 
+    move=> x x' mi @/g /= /mkseqP [i] [rng_i ->] /mkseqP [j] [rng_j ->] /=. 
+    by apply contra => ->.
+  qed.
+  realize dkey_ll by exact: dmkey_ll.
+
 
 (* -- Tweakable Hash Functions -- *)
 (* 
   Tweakable hash function collection that contains all tweakable hash functions
-  used in WOTS-TW, XMSS, and SPHINCS+
+  used in FORS-TW, SPHINCS+ 
 *)
 op thfc : int -> pseed -> adrs -> dgst -> dgstblock.
 
-(* Tweakable hash function used to construct merkle trees from secret values *)
+(* 
+  Tweakable hash function used to produce leaves from secret key values.
+  (Same function as used in chains for WOTS-TW)
+*)
+op f : pseed -> adrs -> dgst -> dgstblock = thfc (8 * n).
+
+clone import TweakableHashFunctions as F with
+  type pp_t <- pseed,
+  type tw_t <- adrs,
+  type in_t <- dgst,
+  type out_t <- dgstblock,
+  
+    op f <- f,
+  
+    op dpp <- dpseed
+    
+  proof *.
+  realize dpp_ll by exact: dpseed_ll.
+
+clone import F.Collection as FC with
+  type diff <- int,
+  
+    op get_diff <- size,
+    
+    op fc <- thfc
+    
+  proof *.
+  realize in_collection by exists (8 * n).
+
+clone import FC.SMDTTCRC as FC_TCR with
+  op t_smdttcr <- d * k * t
+  
+  proof *.
+  realize ge0_tsmdttcr by smt(ge1_d ge1_k ge2_t).
+
+(* Tweakable hash function used to construct Merkle trees from leaves *)
 op trh : pseed -> adrs -> dgst -> dgstblock = thfc (8 * n * 2).
 
 clone import TweakableHashFunctions as TRH with
@@ -349,7 +523,7 @@ clone import TRHC.SMDTTCRC as TRHC_TCR with
   proof *.
   realize ge0_tsmdttcr by smt(ge1_d ge1_k ge2_t).
 
-(* Tweakable hash function used compress merkle tree roots to public key *)
+(* Tweakable hash function used compress Merkle tree roots to public key *)
 op trco : pseed -> adrs -> dgst -> dgstblock = thfc (8 * n * k).
 
 clone import TweakableHashFunctions as TRCO with
@@ -391,7 +565,7 @@ op val_bt_trh (bt : dgstblock bintree) (ps : pseed) (ad : adrs) (hidx : int) (bi
   with bt = Leaf x => x
   with bt = Node l r => 
     trh ps (set_thtbidx ad hidx bidx) 
-      (val (val_bt_trh l ps ad (hidx - 1) (2 * bidx)) ++ val (val_bt_trh r ps ad (hidx - 1) (2 * bidx + 1))).
+        (val (val_bt_trh l ps ad (hidx - 1) (2 * bidx)) ++ val (val_bt_trh r ps ad (hidx - 1) (2 * bidx + 1))).
 
 (* 
   Constructs an authentication path (without embedding it in the corresponding subtype)
@@ -404,7 +578,7 @@ op cons_ap_trh_gen (bt : dgstblock bintree) (bs : bool list) (ps : pseed) (ad : 
   with bt = Node _ _, bs = [] => witness
   with bt = Node l r, bs = b :: bs' =>
     (val_bt_trh (if b then l else r) ps ad (hidx - 1) (if b then 2 * bidx else 2 * bidx + 1)) 
-    :: cons_ap_trh_gen (if b then r else l) bs' ps ad (hidx - 1) (if b then 2 * bidx + 1 else 2 * bidx). 
+     :: cons_ap_trh_gen (if b then r else l) bs' ps ad (hidx - 1) (if b then 2 * bidx + 1 else 2 * bidx). 
 
 (*
   Computes the (hash) value corresponding to an authentication path, a leaf, and a 
@@ -416,28 +590,31 @@ op val_ap_trh_gen (ap : dgstblock list) (bs : bool list) (leaf : dgstblock) (ps 
   with ap = [], bs = _ :: _ => witness 
   with ap = _ :: _, bs = [] => witness
   with ap = x :: ap', bs = b :: bs' =>
-      trh ps (set_thtbidx ad hidx bidx) 
-       (if b 
-        then val x ++ val (val_ap_trh_gen ap' bs' leaf ps ad (hidx - 1) (2 * bidx + 1))
-        else val (val_ap_trh_gen ap' bs' leaf ps ad (hidx - 1) (2 * bidx)) ++ val x).
+    trh ps (set_thtbidx ad hidx bidx) 
+        (if b 
+         then val x ++ val (val_ap_trh_gen ap' bs' leaf ps ad (hidx - 1) (2 * bidx + 1))
+         else val (val_ap_trh_gen ap' bs' leaf ps ad (hidx - 1) (2 * bidx)) ++ val x).
 
 (* 
   Constructs authentication path (embedding it in the corresponding subtype)
   for the special case of binary trees of height a w.r.t. a certain public seed, address, 
-  height index a, and breadth index 0. Expects a binary tree (bt) that is 
-  a merkle tree of height a and index (idx) in [0, 2 ^ a - 1].
+  height index a, and breadth index bidx. Here, idx should be a valid leaf index (i.e., in [0, 2 ^ a -1])
+  and bidx should be a valid breadth index for root nodes of the Merkle trees in a FORS-TW 
+  instance (i.e., in [0, k - 1]).
 *)
-op cons_ap_trh (bt : dgstblock bintree) (idx : int) (ps : pseed) (ad : adrs) : apFORSTW =
-  DBAL.insubd (cons_ap_trh_gen bt (rev (int2bs a idx)) ps ad a 0).
+op cons_ap_trh (bt : dgstblock bintree) (idx : int) (ps : pseed) (ad : adrs) (bidx : int) : apFORSTW =
+  DBAL.insubd (cons_ap_trh_gen bt (rev (int2bs a idx)) ps ad a bidx).
 
 (* 
   Computes value corresponding to an authentication path, leaf, and a path represented 
-  by the big-endian binary representation of an index between 0 (including) 
-  and 2 ^ a (including) w.r.t. a certain public seed, address, height index a, 
-  and breadth index 0. Expects an index (idx) in [0, 2 ^ a - 1].
+  by the big-endian binary representation of an index  w.r.t. a certain public seed, address, 
+  height index a, and breadth index bidx. Here, idx should be a valid leaf index (i.e., in [0, 2 ^ a -1])
+  and bidx should be a valid breadth index for root nodes of the Merkle trees in a FORS-TW 
+  instance (i.e., in [0, k - 1]).
 *)
-op val_ap_trh (ap : apFORSTW) (idx : int) (leaf : dgstblock) (ps : pseed) (ad : adrs) : dgstblock = 
-  val_ap_trh_gen (val ap) (rev (int2bs a idx)) leaf ps ad a 0.
+op val_ap_trh (ap : apFORSTW) (idx : int) (leaf : dgstblock) (ps : pseed) (ad : adrs) (bidx : int) : dgstblock = 
+  val_ap_trh_gen (val ap) (rev (int2bs a idx)) leaf ps ad a bidx.
+
 
 
 (* - Types (3/3) - *)
@@ -461,17 +638,140 @@ clone import Subtype as FAddress with
 type fadrs = FAddress.sT.
 
 
+
 (* - Specification - *)
+(* 
+  Fixed-Length FORS-TW in Encompassing Structure.
+  Addresses given to main procedures (keygen, sign, verify) should be of trhtype
+*)
 module FL_FORS_TW_ES = {
+  proc gen_leaves_single_tree(idxt : int, ss : sseed, ps : pseed, ad : adrs) : dgstblock list = {
+    var skFORS_ele : dgstblock;
+    var leaf : dgstblock;
+    var leaves : dgstblock list;
+    
+    leaves <- [];
+    while (size leaves < t) {
+      skFORS_ele <- skg ss (ps, set_thtbidx ad 0 (idxt * t + size leaves));
+      leaf <- f ps (set_thtbidx ad 0 (idxt * t + size leaves)) (val skFORS_ele);
+      leaves <- rcons leaves leaf;
+    }
+    
+    return leaves;
+  }
+  
+  proc gen_pkFORS(ss : sseed, ps : pseed, ad : adrs) : pkFORS = {
+    var pkFORS : dgstblock;
+    var leaves : dgstblock list;
+    var r : dgstblock;
+    var rs : dgstblock list;
+    var kpidx : int;
+    
+    rs <- [];
+    while (size rs < k) {
+      leaves <@ gen_leaves_single_tree(size rs, ss, ps, ad); 
+      r <- val_bt_trh (list2tree leaves) ps ad a (size rs);
+      rs <- rcons rs r;
+    }
+     
+    pkFORS <- trco ps (set_kpidx (set_typeidx ad trcotype) (get_kpidx ad)) (flatten (map DigestBlock.val rs));
+    
+    return pkFORS;  
+  }
+  
   proc keygen(ss : sseed, ps : pseed, ad : adrs) : pkFORSTW * skFORSTW =  {
-    return witness;
+    var pkFORS : pkFORS;
+    var pk : pkFORSTW;
+    var sk : skFORSTW;
+    
+    pkFORS <@ gen_pkFORS(ss, ps, ad);
+    
+    pk <- (pkFORS, ps, ad);
+    sk <- (ss, ps, ad);
+    
+    return (pk, sk);
   }
   
   proc sign(sk : skFORSTW, m : msgFORSTW) : sigFORSTW = {
-    return witness;
+    var ss : sseed;
+    var ps : pseed;
+    var ad : adrs;
+    var mc : bool list list;
+    var idx : int;
+    var skFORS_ele : dgstblock;
+    var leaves : dgstblock list;
+    var ap : apFORSTW;
+    var sig : (dgstblock * apFORSTW) list;
+    
+    (ss, ps, ad) <- sk;
+    
+    mc <- chunk a (val m);
+    
+    sig <- [];
+    while (size sig < k) {
+      idx <- bs2int (rev (nth witness mc (size sig)));
+      skFORS_ele <- skg ss (ps, set_thtbidx ad 0 (size sig * t + idx));
+      leaves <@ gen_leaves_single_tree(size sig, ss, ps, ad);
+      ap <- cons_ap_trh (list2tree leaves) idx ps ad (size sig);
+      sig <- rcons sig (skFORS_ele, ap);
+    }
+    
+    return insubd sig;
+  }
+  
+  proc pkFORS_from_sigFORSTW(sig : sigFORSTW, m : msgFORSTW, ps : pseed, ad : adrs) : pkFORS = {
+    var skFORS_ele : dgstblock;
+    var ap : apFORSTW;
+    var mc : bool list list;
+    var leaf : dgstblock;
+    var idx : int;
+    var rs : dgstblock list;
+    var root : dgstblock;
+    var pkFORS : pkFORS;
+    
+    mc <- chunk a (val m);
+    
+    rs <- [];
+    while (size rs < k) {
+      idx <- bs2int (rev (nth witness mc (size rs)));
+      (skFORS_ele, ap) <- nth witness (val sig) (size rs);
+      leaf <- f ps (set_thtbidx ad 0 (size rs * t + idx)) (val skFORS_ele);
+      root <- val_ap_trh ap idx leaf ps ad (size rs);
+      rs <- rcons rs root;
+    }
+    
+    pkFORS <- trco ps (set_kpidx (set_typeidx ad trcotype) (get_kpidx ad)) (flatten (map DigestBlock.val rs));
+    
+    return pkFORS;
   }
   
   proc verify(pk : pkFORSTW, m : msgFORSTW, sig : sigFORSTW) : bool = {
+    var ps : pseed;
+    var ad : adrs;
+    var pkFORS, pkFORS' : pkFORS;
+    
+    (pkFORS, ps, ad) <- pk;
+    
+    pkFORS' <@ pkFORS_from_sigFORSTW(sig, m, ps, ad);
+    
+    return pkFORS' = pkFORS;
+  } 
+}.
+
+(* Multi-instance FORS-TW in Encompassing Structure *)
+module M_FORS_TW_ES = {
+  proc keygen(ss : sseed, ps : pseed, ad : adrs) : pkMFORSTW * skMFORSTW =  {
+    
+    return witness;
+  }
+  
+  proc sign(sk : skMFORSTW, m : msg) : sigFORSTW = {
+  
+    return witness;
+  }
+  
+  proc verify(pk : pkMFORSTW, m : msg, sig : sigFORSTW) : bool = {
+  
     return witness;
   } 
 }.
